examples/cellio/CellioAll.v
@@ -1,32 +1,24 @@
 Require Import CRIS Cancel.
 Require Import ImpPrelude.
 Require Import CellioHeader MainHeader InputHeader FooHeader.
-Require Import CellioA CellioI MainA MainI InputA.
+Require Import CellioA CellioI MainA MainI InputA FooA.
 Require Import InputASpec FooASpec.
 Require Import CellioIAproof MainIAproof.
 
 Module CellioAll. Section CellioAll.
-  Import inv_instances.
+  Import inv_instances.  
   Local Instance Γ : HRA := ##[invΓ; CellioAΓ].
   Local Instance Σ : GRA := ##[invΣ; Γ].
-  
-  (* Definition stb_add stb0 stb1: Sk.t -> string -> option fspec :=
-    fun sk fn =>
-      match stb0 sk fn, stb1 sk fn with
-      | Some fsp, None => Some fsp
-      | None, Some fsp => Some fsp
-      | _, _ => None
-      end. *)
-
-  Local Definition smod_src : SMod.t := MainA.Mod ☆ CellioA.Mod ☆ InputA.Mod.
+  Variable foo: Any.t -> itree hmodE Any.t.
+  Local Definition smod_src : SMod.t := MainA.Mod ☆ CellioA.Mod ☆ InputA.Mod ☆ (FooA.Mod foo).
   Local Definition ginv : Sk.t → invspec := λ _ _, True%I.
   Local Definition stb : Sk.t → string → option fspec := stb_global smod_src.
   Local Definition mod_cancel : HMod.t := SModCancel.to_hmod smod_src.
   Local Definition mod_src : HMod.t := SMod.to_hmod ginv stb smod_src.
-  Local Definition mod_tgt : HMod.t := MainI.t ★ CellioI.t ★ (InputA.t ginv stb).
+  Local Definition mod_tgt : HMod.t := MainI.t ★ CellioI.t ★ (InputA.t ginv stb) ★ (FooA.t foo ginv stb).
 
   Local Definition main_fsp : fspec := fspec_trivial.
-  Local Definition init_cond : Sk.t → iProp Σ := MainA.InitCond ∗∗ CellioA.InitCond ∗∗ InputA.InitCond.
+  Local Definition init_cond : Sk.t → iProp Σ := MainA.InitCond ∗∗ CellioA.InitCond ∗∗ InputA.InitCond ∗∗ FooA.InitCond.
   Local Definition skeleton : Sk.t := Sk.add CellioSK.t MainSK.t.
 
   (* Apply cancellation to linked spec module *)
@@ -42,10 +34,12 @@ Module CellioAll. Section CellioAll.
   (* Refinement between spec/impl of whole program (linked module) *)
   Lemma src_tgt : refines (mod_src, init_cond) (mod_tgt, const(emp)%I).
   Proof.
-    (* consider identical modules in src/tgt as context (InputA) *)
+    (* consider identical modules in src/tgt as context (InputA, FooA) *)
     eapply ctxr_refines.
-    rewrite -[(_, const (emp%I))]hmod_addc_empty_r /init_cond -hmod_addc_assoc.
-    rewrite /mod_src /mod_tgt !add_interp_comm -!hmod_add_assoc /InputA.t.
+    rewrite -[(_, const (emp%I))]hmod_addc_empty_r /init_cond -!hmod_addc_assoc.
+    rewrite /mod_src /mod_tgt !add_interp_comm -!hmod_add_assoc /FooA.t.
+    unseal CRIS. eapply ctxr_frameR, ctxr_cond_frameR.
+    rewrite -[(_, const (emp%I))]hmod_addc_empty_r /InputA.t.
     unseal CRIS. eapply ctxr_frameR, ctxr_cond_frameR.
     (* solve by transitivity:
       MainI ★ CellioI ⊆ MainI ★ CellioA ⊆ MainA ★ CellioA 
@@ -57,7 +51,8 @@ Module CellioAll. Section CellioAll.
       instantiate (1:= (MainI.t ★ (CellioA.t ginv stb), (const(emp%I)) ∗∗ CellioA.InitCond)).
       eapply ctxr_cond_frameR, main_adequacy, MainIA.sim.
       {
-        admit. 
+        i. rewrite /FooAS.Stb. unseal CRIS. econs; first prove_nodup.
+        ii; rewrite -FIND /stb /stb_global /smod_src //=. des_ifs; ss; des_ifs.
       }
       {
         i. rewrite /InputAS.Stb. unseal CRIS. econs; first prove_nodup.
@@ -71,8 +66,7 @@ Module CellioAll. Section CellioAll.
     i. rewrite /InputAS.Stb. unseal CRIS. econs; first prove_nodup.
     ii; rewrite -FIND /stb /stb_global /smod_src //=.
     des_ifs; ss; des_ifs.
-  (* Qed. *)
-  Admitted.
+  Qed.
 
   Lemma cancel_tgt :
     refines (mod_cancel, init_cond ∗∗ (λ _, main_fsp.(precond) 0 tt tt↑ tt↑))
@@ -83,12 +77,13 @@ Module CellioAll. Section CellioAll.
     { eapply src_tgt. }
   Qed.
 
-  Local Definition initial_resource : Σ := MainAS.init_res ⋅ CellioAS.init_res.
+  Local Definition initial_resource : Σ := MainA.InitRes ⋅ CellioA.InitRes ⋅ InputA.InitRes ⋅ FooA.InitRes.
+
   Lemma initial_resource_valid : ✓ initial_resource.
   Proof.
-    rewrite /initial_resource /MainAS.init_res /CellioAS.init_res -own.iRes_singleton_op.
-    apply discrete_fun_singleton_valid, allocs.allocs_frag_valid,
-      cmra_transport_valid, excl_auth_valid.
+    rewrite /initial_resource /CellioA.InitRes !right_id left_id /own.iRes_singleton.
+    apply discrete_fun_singleton_valid, allocs.allocs_frag_valid, cmra_transport_valid. 
+    unfold "●E". apply auth_auth_valid. econs.  
   Qed.
 
   Theorem behavioral_refinement :
@@ -98,16 +93,17 @@ Module CellioAll. Section CellioAll.
   Proof.
     move: (cancel_tgt)=>H; rewrite /refines in H; des; ss.
     destruct (REF skeleton initial_resource).
-    { rewrite /CellioI.t /MainI.t /skeleton; unseal CRIS; ss. }
+    { rewrite /CellioI.t /MainI.t /InputA.t /FooA.t /skeleton; unseal CRIS; ss. }
     { rewrite /skeleton /CellioSK.t /MainSK.t; ss; econs; ii; ss; des; ss; prove_nodup. }
     { apply initial_resource_valid. }
-    { iIntros "I"; rewrite /init_cond /CellioA.init_cond /MainA.init_cond /HMod.addc.
-      rewrite /precond /= /CellioAS.Ready /CellioAS.Ball
-        own.Own_eq own.own_eq /own.Own_def /own.own_def.
-      iDestruct "I" as "[I1 I2]"; iFrame. iSplit; iPureIntro; ss.
+    { iIntros "I"; rewrite /init_cond /CellioA.InitCond /MainA.InitCond /InputA.InitCond /FooA.InitCond /HMod.addc.
+      rewrite /precond /= /CellioA.auth 
+       own.Own_eq own.own_eq /own.Own_def /own.own_def. 
+      iDestruct "I" as "[[[_ I] _] _]"; iFrame. 
+      iSplit; iPureIntro; ss.
     }
     { econs; ss; try prove_nodup. }
     { exists x; des; eauto. }
   Qed.
 End CellioAll. End CellioAll.
-Print Assumptions CellioAll.behavioral_refinement.
+(* Print Assumptions CellioAll.behavioral_refinement. *)
