examples/cellio/FooA.v
@@ -1,0 +1,65 @@
+Require Import CRIS.
+Require Import MainHeader CellioHeader InputHeader FooHeader.
+
+Require Import CellioA MainA InputA.
+
+Set Implicit Arguments.
+
+Module FooA. Section FooA.
+  Context `{Σ: GRA}.
+  (* Context `{!invG α Σ Γ, !subHG Γ Σ, !sinvG Σ Γ α β τ, !CellioAGΓ Γ}. *)
+  
+  (* Unknown function body. Shouldn't call functions in local modules *)
+  Variable foo: Any.t -> itree hmodE Any.t.
+  (* 
+    need some better idea to specify the list of local function names 
+    without linking all local modules at this moment.
+  *)
+  (* Local Definition modules := (CellioA.t ginv GlobalStb) ★ (MainA.t ginv GlobalStb) ★ (InputA.t ginv GlobalStb). *)  
+  Local Definition local_fns 
+    := [CellioName.set; CellioName.get; MainName.main; InputName.input].
+
+  Local Definition handle_call: callE ~> itree hmodE :=
+    λ _ '(Call fn varg), 
+      match (existsb (String.eqb fn) local_fns) with
+      | true => trigger (Call fn varg)
+      | false => triggerUB
+      end.
+
+  Local Definition interp_body R (it : itree hmodE R) : itree hmodE R :=
+    interp (case_ (bif:=sum1) trivial_Handler
+           (case_ (bif:=sum1) trivial_Handler
+           (case_ (bif:=sum1) handle_call
+                              trivial_Handler))) it.
+
+  Local Definition interp_fun (f : Any.t -> itree hmodE Any.t) : Any.t -> itree hmodE Any.t :=
+    λ x, interp_body (f x).
+
+  Definition scopes := [FooName.mn].
+  
+  Definition fnsems : alist string (list string * fspecbody) :=
+    [(FooName.foo, (scopes, mk_specbody fspec_trivial (interp_fun foo)))].
+
+  Program Definition Sem : SModSem.t := {|
+    SModSem.scopes := scopes;
+    SModSem.fnsems := fnsems;
+    SModSem.initial_st := [];
+  |}.
+  Solve All Obligations with prove_scope.
+  Next Obligation. prove_nodup. Qed.
+
+  Definition Mod : SMod.t := {|
+    SMod.modsem := λ _, Sem;
+    SMod.sk := FooSK.t;
+  |}.
+
+  Definition InitCond : Sk.t -> iProp Σ :=
+    λ _, emp%I.
+
+  Definition InitRes : Σ := ε.
+
+  Variable ginv: Sk.t -> invspec.
+  Variable GlobalStb: Sk.t -> string -> option fspec.
+
+  Definition t := Seal.sealing CRIS (SMod.to_hmod ginv GlobalStb Mod).
+End FooA. End FooA.
